MLS.Parser.fsti
@@ -4,6 +4,11 @@ open MLS.Bytes
 
 (*** Basic definitions ***)
 
+let rec for_allP (#a:Type) (pre:a -> Type0) (l:list a): Type0 =
+    match l with
+    | [] -> True
+    | h::t -> pre h /\ for_allP pre t
+
 val add_prefixes: #bytes:Type0 -> {|bytes_like bytes|} -> list (bytes) -> bytes -> bytes
 
 /// What is the reason behind `parser_serializer_unit` and `parser_serializer`?
@@ -49,7 +54,7 @@ noeq type parser_serializer_unit (bytes:Type0) {|bytes_like bytes|} (a:Type) = {
     | None -> True
   );
   serialize_pre: pre:bytes_compatible_pre bytes -> x:a{is_valid pre x} -> Lemma (
-    forall b. List.Tot.memP b (serialize x) ==> pre b
+    for_allP pre (serialize x)
   )
 }
 
@@ -62,12 +67,27 @@ val bind: #a:Type -> #b:(a -> Type) -> #bytes:Type0 -> {| bytes_like bytes |} ->
   (requires True)
   (ensures fun res -> is_not_unit res <==> is_not_unit ps_a \/ (forall xa. is_not_unit (ps_b xa)))
 
+val bind_is_valid:
+  #a:Type -> #b:(a -> Type) -> #bytes:Type0 -> {| bytes_like bytes |} ->
+  ps_a:parser_serializer_unit bytes a -> ps_b:(xa:a -> parser_serializer_unit bytes (b xa)) ->
+  pre:bytes_compatible_pre bytes -> xa:a -> xb:(b xa) ->
+  Lemma ((bind ps_a ps_b).is_valid pre (|xa, xb|) <==> ps_a.is_valid pre xa /\ (ps_b xa).is_valid pre xb)
+  [SMTPat ((bind ps_a ps_b).is_valid pre (|xa, xb|))]
+
 val isomorphism_explicit:
   #a:Type -> #bytes:Type0 -> {| bytes_like bytes |} -> b:Type ->
   ps_a:parser_serializer_unit bytes a -> f:(a -> b) -> g:(b -> a) ->
   g_f_inv:(xa:a -> Lemma (g (f xa) == xa)) -> f_g_inv:(xb:b -> Lemma (f (g xb) == xb)) ->
   Pure (parser_serializer_unit bytes b) (requires True)
   (ensures fun res -> is_not_unit res <==> is_not_unit ps_a)
+
+val isomorphism_explicit_is_valid:
+  #a:Type -> #bytes:Type0 -> {| bytes_like bytes |} -> b:Type ->
+  ps_a:parser_serializer_unit bytes a -> f:(a -> b) -> g:(b -> a) ->
+  g_f_inv:(xa:a -> Lemma (g (f xa) == xa)) -> f_g_inv:(xb:b -> Lemma (f (g xb) == xb)) ->
+  pre:bytes_compatible_pre bytes -> xb:b ->
+  Lemma ((isomorphism_explicit b ps_a f g g_f_inv f_g_inv).is_valid pre xb <==> ps_a.is_valid pre (g xb))
+  [SMTPat ((isomorphism_explicit b ps_a f g g_f_inv f_g_inv).is_valid pre xb)]
 
 val isomorphism:
   #a:Type -> #bytes:Type0 -> {| bytes_like bytes |} -> b:Type ->
@@ -76,10 +96,25 @@ val isomorphism:
   (requires (forall xa. g (f xa) == xa) /\ (forall xb. f (g xb) == xb))
   (ensures fun res -> is_not_unit res <==> is_not_unit ps_a)
 
+val isomorphism_is_valid:
+  #a:Type -> #bytes:Type0 -> {| bytes_like bytes |} -> b:Type ->
+  ps_a:parser_serializer_unit bytes a -> f:(a -> b) -> g:(b -> a) ->
+  pre:bytes_compatible_pre bytes -> xb:b ->
+  Lemma (requires (forall xa. g (f xa) == xa) /\ (forall xb. f (g xb) == xb))
+  (ensures (isomorphism b ps_a f g).is_valid pre xb <==> ps_a.is_valid pre (g xb))
+  [SMTPat ((isomorphism b ps_a f g).is_valid pre xb)]
+
 (*** Parser for basic types ***)
 
 val ps_unit: #bytes:Type0 -> {| bytes_like bytes |} -> Pure (parser_serializer_unit bytes unit) (requires True)
   (ensures fun res -> forall pre x. res.is_valid pre x)
+
+val ps_unit_is_valid:
+  #bytes:Type0 -> {| bl:bytes_like bytes |} ->
+  pre:bytes_compatible_pre bytes -> x:unit ->
+  Lemma ((ps_unit #bytes #bl).is_valid pre x <==> True)
+  [SMTPat ((ps_unit #bytes #bl).is_valid pre x)]
+
 
 type lbytes (bytes:Type0) {|bytes_like bytes|} (n:nat) = b:bytes{length b == n}
 val ps_lbytes: #bytes:Type0 -> {| bytes_like bytes |} -> n:nat -> Pure (parser_serializer_unit bytes (lbytes bytes n))
@@ -89,6 +124,13 @@ val ps_lbytes: #bytes:Type0 -> {| bytes_like bytes |} -> n:nat -> Pure (parser_s
   ) /\ (
     forall (pre:bytes_compatible_pre bytes) b. res.is_valid pre b <==> pre b
   ))
+
+val ps_lbytes_is_valid:
+  #bytes:Type0 -> {| bytes_like bytes |} -> n:nat ->
+  pre:bytes_compatible_pre bytes -> x:lbytes bytes n ->
+  Lemma ((ps_lbytes n).is_valid pre x <==> pre (x <: bytes))
+  [SMTPat ((ps_lbytes n).is_valid pre x)]
+
 
 //val ps_u8: parser_serializer uint8
 //val ps_u16: parser_serializer uint16
@@ -122,7 +164,22 @@ noeq type parser_serializer_exact (bytes:Type0) {|bytes_like bytes|} (a:Type) = 
 }
 
 val ps_to_pse: #bytes:Type0 -> {|bytes_like bytes|} -> #a:Type -> parser_serializer_unit bytes a -> parser_serializer_exact bytes a
+
+val ps_to_pse_is_valid:
+  #bytes:Type0 -> {|bytes_like bytes|} -> #a:Type ->
+  ps_a:parser_serializer_unit bytes a ->
+  pre:bytes_compatible_pre bytes -> x:a ->
+  Lemma ((ps_to_pse ps_a).is_valid_exact pre x <==> ps_a.is_valid pre x)
+  [SMTPat ((ps_to_pse ps_a).is_valid_exact pre x)]
+
 val pse_list: #bytes:Type0 -> {|bytes_like bytes|} -> #a:Type -> ps_a:parser_serializer bytes a -> parser_serializer_exact bytes (list a)
+
+val pse_list_is_valid:
+  #bytes:Type0 -> {|bytes_like bytes|} -> #a:Type ->
+  ps_a:parser_serializer bytes a ->
+  pre:bytes_compatible_pre bytes -> l:list a ->
+  Lemma ((pse_list ps_a).is_valid_exact pre l <==> for_allP (ps_a.is_valid pre) l)
+  [SMTPat ((pse_list ps_a).is_valid_exact pre l)]
 
 (*** Parser for variable-length lists ***)
 
@@ -139,5 +196,20 @@ let bytes_length (#bytes:Type0) {|bytes_like bytes|} (#a:Type) (ps_a:parser_seri
 
 type blseq (#bytes:Type0) {|bytes_like bytes|} (a:Type) (ps_a:parser_serializer bytes a) (r:size_range) = s:Seq.seq a{in_range r (bytes_length ps_a (Seq.seq_to_list s))}
 type blbytes (bytes:Type0) {|bytes_like bytes|} (r:size_range) = b:bytes{in_range r (length b)}
+
 val ps_seq: #bytes:Type0 -> {|bytes_like bytes|} -> #a:Type -> r:size_range -> ps_a:parser_serializer bytes a -> parser_serializer bytes (blseq a ps_a r)
+
+val ps_seq_is_valid:
+  #bytes:Type0 -> {|bytes_like bytes|} -> #a:Type ->
+  r:size_range -> ps_a:parser_serializer bytes a ->
+  pre:bytes_compatible_pre bytes -> x:blseq a ps_a r ->
+  Lemma ((ps_seq r ps_a).is_valid pre x <==> for_allP (ps_a.is_valid pre) (Seq.seq_to_list x))
+  [SMTPat ((ps_seq r ps_a).is_valid pre x)]
+
 val ps_bytes: #bytes:Type0 -> {|bytes_like bytes|} -> r:size_range -> parser_serializer bytes (blbytes bytes r)
+
+val ps_bytes_is_valid:
+  #bytes:Type0 -> {|bytes_like bytes|} -> r:size_range ->
+  pre:bytes_compatible_pre bytes -> x:blbytes bytes r ->
+  Lemma ((ps_bytes r).is_valid pre x <==> pre x)
+  [SMTPat ((ps_bytes r).is_valid pre x)]
